Precondition_Normalization/Precondition_Normalization.thy
@@ -6,52 +6,156 @@ section \<open> Precondition Normalization Well-Formedness Proofs \<close>
 
 subsection \<open> Action splitting properties \<close>
 
-lemma (in ast_classical_domain) split_ac_len:
-  "length (split_ac ac) = length (dnf_list (ac_pre ac))"
+lemma is_conj_preprend_atoms_to_conj:
+  assumes "is_conj f"
+  shows "is_conj (prepend_atoms_to_conj as f)"
+  using assms apply (induction as arbitrary: f) 
+  by (auto simp: prepend_atoms_to_conj_def)
+
+lemma pne_equiv_dnf_list_length[simp]:
+  "length (pne_equiv_dnf_list f) = length (dnf_list f)"
+  unfolding pne_equiv_dnf_list_def by simp
+
+lemma pne_equiv_dnf_list_conjs:
+  "\<forall>f \<in> set (pne_equiv_dnf_list F). is_conj f"
+  unfolding pne_equiv_dnf_list_def Let_def 
+  using dnf_list_conjs is_conj_preprend_atoms_to_conj by auto
+
+lemma atoms_prepend_atoms_to_conj[simp]:
+  "atoms (prepend_atoms_to_conj as f) = set as \<union> atoms f"
+  unfolding prepend_atoms_to_conj_def by (induction as) auto
+
+lemma formula_enum_pnes_prepend_atoms_to_conj:
+  "set (formula_enumerate_primitive_numeric_expressions (prepend_atoms_to_conj as f))
+   = (\<Union>a \<in> set as. set (atom_enumerate_primitive_numeric_expressions a))
+     \<union> set (formula_enumerate_primitive_numeric_expressions f)"
+  unfolding prepend_atoms_to_conj_def by (induction as) auto
+
+lemma predAtm_notin_pnes_def_checks: "predAtm p xs \<notin> set (pnes_def_checks f)"
+  unfolding pnes_def_checks_def Let_def by auto
+
+lemma eqAtm_notin_pnes_def_checks: "eqAtm a b \<notin> set (pnes_def_checks f)"
+  unfolding pnes_def_checks_def Let_def by auto
+
+(* the definedness checks enumerate exactly the pnes of the original formula *)
+lemma pnes_of_pnes_def_checks:
+  "(\<Union>a \<in> set (pnes_def_checks f). set (atom_enumerate_primitive_numeric_expressions a))
+   = set (formula_enumerate_primitive_numeric_expressions f)"
+  unfolding pnes_def_checks_def Let_def by auto
+
+lemma pne_equiv_dnf_list_decomp:
+  assumes "g \<in> set (pne_equiv_dnf_list f)"
+  obtains c where "c \<in> set (dnf_list f)"
+    and "g = prepend_atoms_to_conj (pnes_def_checks f) c"
+  using assms by (auto simp: pne_equiv_dnf_list_def Let_def)
+
+text \<open>For each clause of \<open>pne_equiv_dnf_list\<close>, the prepended definedness checks
+  restore exactly the primitive numeric expressions of the original precondition,
+  whereas its predicate and equality atoms can only shrink (they all stem from one
+  DNF clause of the original formula).\<close>
+
+(* pnes: every clause enumerates exactly the pnes of the original formula *)
+lemma pne_equiv_dnf_list_pnes:
+  assumes "g \<in> set (pne_equiv_dnf_list f)"
+  shows "set (formula_enumerate_primitive_numeric_expressions g)
+       = set (formula_enumerate_primitive_numeric_expressions f)"
+proof -
+  from assms obtain c where c: "c \<in> set (dnf_list f)"
+    and g: "g = prepend_atoms_to_conj (pnes_def_checks f) c"
+    by (rule pne_equiv_dnf_list_decomp)
+  have "atoms c \<subseteq> atoms f" using c dnf_list_atoms by fast
+  hence sub: "set (formula_enumerate_primitive_numeric_expressions c)
+       \<subseteq> set (formula_enumerate_primitive_numeric_expressions f)"
+    by (auto simp: set_formula_enumerate_primitive_numeric_expressions_conv)
+  show ?thesis
+    unfolding g formula_enum_pnes_prepend_atoms_to_conj pnes_of_pnes_def_checks
+    using sub by auto
+qed
+
+(* predicate atoms: every clause's predicate atoms come from the original formula *)
+lemma pne_equiv_dnf_list_predAtm:
+  assumes "g \<in> set (pne_equiv_dnf_list f)" and "predAtm p xs \<in> atoms g"
+  shows "predAtm p xs \<in> atoms f"
+proof -
+  from assms(1) obtain c where c: "c \<in> set (dnf_list f)"
+    and g: "g = prepend_atoms_to_conj (pnes_def_checks f) c"
+    by (rule pne_equiv_dnf_list_decomp)
+  from assms(2)[unfolded g]
+  have "predAtm p xs \<in> set (pnes_def_checks f) \<union> atoms c" by simp
+  hence "predAtm p xs \<in> atoms c" using predAtm_notin_pnes_def_checks by blast
+  thus "predAtm p xs \<in> atoms f" using c dnf_list_atoms by fast
+qed
+
+(* equality atoms: every clause's equality atoms come from the original formula *)
+lemma pne_equiv_dnf_list_eqAtm:
+  assumes "g \<in> set (pne_equiv_dnf_list f)" and "eqAtm a b \<in> atoms g"
+  shows "eqAtm a b \<in> atoms f"
+proof -
+  from assms(1) obtain c where c: "c \<in> set (dnf_list f)"
+    and g: "g = prepend_atoms_to_conj (pnes_def_checks f) c"
+    by (rule pne_equiv_dnf_list_decomp)
+  from assms(2)[unfolded g]
+  have "eqAtm a b \<in> set (pnes_def_checks f) \<union> atoms c" by simp
+  hence "eqAtm a b \<in> atoms c" by (simp add: eqAtm_notin_pnes_def_checks)
+  thus "eqAtm a b \<in> atoms f" using c dnf_list_atoms by fast
+qed
+
+
+lemma (in ast_classical_domain) split_ac_names_length:
   "length (split_ac_names ac) = length (dnf_list (ac_pre ac))"
-  unfolding split_ac_def split_ac_names_def n_clauses_def by simp_all
+  unfolding split_ac_names_def length_map n_clauses_def by simp
+
+lemma (in ast_classical_domain) split_ac_length:
+  "length (split_ac ac) = length (dnf_list (ac_pre ac))"
+  unfolding split_ac_def 
+  unfolding Let_def length_map2 
+  unfolding pne_equiv_dnf_list_length split_ac_names_length
+  by force
+
 
 lemma (in ast_classical_domain) split_ac_nth:
   assumes "i < length (dnf_list (ac_pre ac))"
   shows "split_ac ac ! i =
     SimpleActionSchema
       (ActionHead (padl_lit split_pre_pad (String.implode (show i)) + ac_name ac) (ac_params ac))
-      (SimpleActionBody (dnf_list (ac_pre ac) ! i) (ac_eff ac))"
+      (SimpleActionBody (pne_equiv_dnf_list (ac_pre ac) ! i) (ac_eff ac))"
   using assms unfolding split_ac_def split_ac_names_def n_clauses_def
   apply (induction ac rule: ast_classical_action_schema_induct_unfold) 
-  by (simp add: padl_lit_implode)
+  by (simp add: padl_lit_implode pne_equiv_dnf_list_length)
 
 lemma (in ast_classical_domain4) p_ac:
   "ac' \<in> set (actions D4) \<longleftrightarrow> (\<exists>ac \<in> set (actions D). ac' \<in> set (split_ac ac))"
   unfolding split_dom_sel split_acs_def by simp
 
-lemma (in ast_classical_domain) split_pres: "map ac_pre (split_ac a) = dnf_list (ac_pre a)"
-  unfolding split_ac_def Let_def apply (rule set_n_pre_mapsel)
-  unfolding split_ac_names_def n_clauses_def by simp
+lemma (in ast_classical_domain) split_pres: 
+  "map ac_pre (split_ac a) = pne_equiv_dnf_list (ac_pre a)"
+  unfolding split_ac_def Let_def 
+  apply (rule set_n_pre_mapsel)
+  using split_ac_names_length by simp
 
 lemma (in ast_classical_domain) split_ac_sel:
   assumes "a' \<in> set (split_ac a)"
   shows
     "\<exists>i < length (split_ac a). ac_name a' = padl_lit split_pre_pad (String.implode (show i)) + ac_name a"
     "ac_params a' = ac_params a"
-    "ac_pre a' \<in> set (dnf_list (ac_pre a))"
+    "ac_pre a' \<in> set (pne_equiv_dnf_list (ac_pre a))"
     "ac_eff a' = ac_eff a"
 proof -
   from assms show "ac_params a' = ac_params a" "ac_eff a' = ac_eff a"
     unfolding split_ac_def Let_def by auto
   from assms obtain i where i: "i < length (split_ac a)" "a' = split_ac a ! i"
     using in_set_conv_nth by metis
-  from i show "ac_pre a' \<in> set (dnf_list (ac_pre a))"
-    using split_ac_nth split_ac_len(1) by simp
+  from i show "ac_pre a' \<in> set (pne_equiv_dnf_list (ac_pre a))"
+    using split_ac_nth[of i a] split_ac_length split_ac_names_length by auto
   from i show "\<exists>i < length (split_ac a). ac_name a' = padl_lit split_pre_pad (String.implode (show i)) + ac_name a"
-    using split_ac_nth split_ac_len(1) by auto
+    using split_ac_nth split_ac_names_length split_ac_length by auto
 qed
 
 subsection \<open> Output format \<close>
 
 theorem (in ast_classical_problem4) prec_normed_ac:
   "\<forall>ac' \<in> set (split_ac ac). is_conj (ac_pre ac')"
-  using split_ac_sel(3) dnf_list_conjs by auto
+  using split_ac_sel(3) pne_equiv_dnf_list_conjs by auto
 
 theorem (in ast_classical_problem4) prec_normed_dom:
   "d4.prec_normed_dom"
@@ -173,9 +277,12 @@ lemma p_actions_wf: "list_all d4.wf_classical_action_schema (actions D4)"
 proof (subst list_all_iff, intro ballI)
   fix a' assume assm: "a' \<in> set (actions D4)"
   then obtain a where a: "a \<in> set (actions D)" "a' \<in> set (split_ac a)" using p_ac by auto
-  hence "atoms (ac_pre a') \<subseteq> atoms (ac_pre a)" using split_ac_sel(3) dnf_list_atoms by metis
-  hence fmla_wf: "d4.wf_fmla tyt (ac_pre a')" if "wf_fmla tyt (ac_pre a)" for tyt
-    using that wf_fmla_alt by blast
+  have fmla_wf: "d4.wf_fmla tyt (ac_pre a')" if "wf_fmla tyt (ac_pre a)" for tyt
+    apply (rule d4.wf_fmlaI)
+    using wf_fmla_imp_wf_pred_atom[OF that] wf_fmla_imp_eqs_def[OF that] wf_fmla_imp_wf_pnes[OF that]
+    by (force simp: pne_equiv_dnf_list_pnes[OF split_ac_sel(3)[OF a(2)]] 
+     dest!: pne_equiv_dnf_list_eqAtm[OF split_ac_sel(3)[OF a(2)]]
+     pne_equiv_dnf_list_predAtm[OF split_ac_sel(3)[OF a(2)]])+
 
   have ac_tyt: "ac_tyt a' = ac_tyt a" 
     using split_ac_sel[OF a(2)] ac_tyt_def by simp
@@ -203,5 +310,7 @@ sublocale wf_ast_classical_domain4 \<subseteq> wf_ast_classical_domain D4
 
 sublocale wf_ast_classical_problem4 \<subseteq> p4_wf: wf_ast_classical_problem P4
   using split_prob_wf wf_ast_classical_problem.intro by simp_all
+
+
 
 end
